src/coq/polyir/PolyIRDefinition.v
@@ -359,33 +359,47 @@ Fixpoint option_traverse {A: Type} (lo: list (option A)): option (list A) :=
   | oa::lo' => oa >>= (fun a => option_map (cons a) (option_traverse lo'))
   end.
 
+
+
+Fixpoint option_traverse_fold_left {ACCUM A: Type}
+         (accum: ACCUM)
+         (f: ACCUM -> A -> option ACCUM)
+         (l: list A): option (ACCUM) :=
+  match l with
+  | [] => Some accum
+  | a::l' => (f accum a) >>= (fun accum2 => option_traverse_fold_left accum2 f l')
+  end.
+
 Module Type POLYHEDRAL_THEORY.
   Parameter PointT: Type.
   Parameter PolyT: Type.
   Parameter AffineFnT: Type.
   Parameter AffineRelT: Type.
   Parameter ParamsT: Type.
-  (* Some way to specify a dimension *)
+  (** Some way to specify a dimension *)
   Parameter DimensionT: Type.
-  (* Some way to map a point with an affine function *)
+  (** Some way to map a point with an affine function *)
   Parameter mapPoint: AffineFnT -> PointT -> option (PointT).
-  (* Has some way to fill in the free variables *)
+  (** Has some way to fill in the free variables *)
   Parameter evalPoint: ParamsT -> PointT -> option (list Z).
-  (* Have some way to compose affine functions *)
+  (** Have some way to compose affine functions *)
   Parameter composeAffineFunction: AffineFnT -> AffineFnT -> option AffineFnT.
-  (* Compute the inverse of an affine function *)
+  (** Compute the inverse of an affine function *)
   Parameter invertAffineFunction: AffineFnT -> option AffineFnT.
-  (* Have some way to check if two points are related *)
+  (** Have some way to check if two points are related *)
   Parameter arePointsRelated: PointT -> PointT -> AffineRelT -> bool.
-  (* Check if a point is within a polyhedra *)
+  (** Check if a point is within a polyhedra *)
   Parameter isPointInPoly: PointT -> PolyT -> bool.
 
-  (* Returns whether one point is lex smaller than the other *)
+  (** Returns whether one point is lex smaller than the other *)
   Parameter isLexSmaller: PointT -> PointT -> option (bool).
 
-  (* Find the next point that is within the polyhedra which is
+  (** Returns whether one point is lex smaller than the other *)
+  Parameter getLexminPoint: ParamsT -> PolyT -> PointT.
+
+  (** Find the next point that is within the polyhedra which is
     one larger in terms of lex order. return Nothing if not possible *)
-  Parameter getNextLexLargerPoint: ParamsT ->
+  Parameter getNextLexPoint: ParamsT ->
                                    PolyT ->
                                    PointT ->
                                    option (PointT).
@@ -393,20 +407,20 @@ Module Type POLYHEDRAL_THEORY.
   Parameter getOverapproximationNumPointsInPoly: ParamsT ->
                                                  PolyT ->
                                                  option (nat).
-  (* Definition of an empty polyhedra *)
+  (** Definition of an empty polyhedra *)
   Parameter emptyPoly: PolyT.
 
-  (* Empty affine relation *)
+  (** Empty affine relation *)
   Parameter emptyAffineRel: AffineRelT.
 
-  (* Take a union of two relations *)
+  (** Take a union of two relations *)
   Parameter unionAffineRel:  AffineRelT -> AffineRelT -> AffineRelT.
 
-  (* Weaken an affine function into an affine relation *)
+  (** Weaken an affine function into an affine relation *)
   Parameter affineFnToAffineRel: AffineFnT -> AffineRelT.
 
 
-  (* Definition of union of polyhedra *)
+  (** Definition of union of polyhedra *)
   Parameter unionPoly:  PolyT -> PolyT -> option PolyT.
 
   (** Defines what it means to be a dependence relation. This is the
@@ -417,7 +431,7 @@ Module Type POLYHEDRAL_THEORY.
         t1 < t2
         ===============
           t1 --D--> t2
-   **)
+   *)
   Definition relationIsDependenceBetweenRelations
              (r1 r2: AffineRelT)
              (dep: AffineRelT): Prop :=
@@ -428,7 +442,7 @@ Module Type POLYHEDRAL_THEORY.
            (TP_LEX_ORDERED: isLexSmaller tp1 tp2 = Some true),
       arePointsRelated tp1 tp2 dep = true.
 
-  (* A function to compute the dependence polyhedra of two relations *)
+  (** A function to compute the dependence polyhedra of two relations *)
   Parameter getDependenceRelation: AffineRelT -> AffineRelT -> option AffineRelT.
   
   
@@ -444,15 +458,18 @@ Module SCOP(P: POLYHEDRAL_THEORY).
    *)
 
 
-  Inductive ScopStmtType :=
-  | SSTstore: (list Value -> Value) (* Value to store; this is temporary *)
-              -> ScopStmtType
-  | SSTload: ScopStmtType.
+  Definition AccessFunction := P.AffineFnT. (**r Access function to model where to read or write from *)
+  Inductive MemoryAccess :=
+  | MAStore: Ident (**r name *)
+                    -> AccessFunction
+                    -> (list Value -> Value) (**r value *)    
+                    -> MemoryAccess
+  | MALoad: Ident (**r name *)
+                   -> AccessFunction
+                   -> MemoryAccess.
 
   Record ScopEnvironment :=
     mkScopEnvironment {
-        (* VIV = virtual induction variable *)
-        scopenvVIV: P.PointT;
         scopenvParams: P.ParamsT;
         scopenvIdentToChunkNum: ZMap.t (option ChunkNum);
       }.
@@ -462,29 +479,17 @@ conceptually, we don't actually care either. We just want to make sure
 that the reads/writes are modeled *)
   Record ScopStmt :=
     mkScopStmt {
-        (** Identifier of the scop statement *)
-        scopStmtArrayIdent : Ident;
-        (** The domain of the scop statement. That is, interpreted as
-          0 <= <indvars[i]> <= <domain[i]> **)
-        scopStmtDomain: P.PolyT;
-        (** Function from the canonical induction variables to the schedule
-         timepoint. That is, interpreted as the output dimensions when
-         invoked against the input **)
-        (** Note that the schedule dimensions can be larger than the input
-      dimension **)
-        scopStmtSchedule : P.AffineFnT;
-        (** Access function to model where to read or write from **)
-        scopStmtAccessFunction: P.AffineFnT;
-        (** Type of the scop statement: store or load **)
-        scopStmtType: ScopStmtType
+        scopStmtDomain: P.PolyT; (**r The domain of the scop statement. That is, interpreted as
+          0 <= <indvars[i]> <= <domain[i]> *)
+        scopStmtSchedule : P.AffineFnT; (**r Function from the canonical induction variables to the schedule
+         timepoint.  *)
+        scopStmtMemAccesses: list MemoryAccess (**r List of memory accesses *)
       }.
 
   Record Scop :=
     mkScop {
-        (** The statements in this scop **)
-        scopStmts : list ScopStmt;
-        (** Induction variables in this scop **)
-        scopIndvars : list P.DimensionT;
+        scopStmts : list ScopStmt; (**r The statements in this scop *)
+        scopIndvars : list P.DimensionT; (**r Induction variables in this scop *)
       }.
 
   Fixpoint all (bs: list bool): bool :=
@@ -506,10 +511,6 @@ that the reads/writes are modeled *)
              (ys: list Y): list (X * Y) :=
     @zipWith X Y (X * Y) (fun x y => (x, y)) xs ys.
 
-  (* Check if the current value of the induction variables is within
-the scop stmts domain *)
-  Definition isScopStmtActive (se: ScopEnvironment) (ss: ScopStmt) : bool :=
-    P.isPointInPoly (scopenvVIV se) (scopStmtDomain ss).
 
   (* Build on the abstraction of memory to store into an array *)
   Definition storeArray (arrayIdent: Ident)
@@ -521,92 +522,10 @@ the scop stmts domain *)
     | Some chnk => storeMemory chnk ix val mem
     | None => mem
     end.
-  
-  
 
-  (** TODO: make loads an actual statement in the PolyIR language **)
-  Definition runScopStmt (ss: ScopStmt)
-             (se: ScopEnvironment)
-             (mem: Memory) : Memory :=
-    (* let oaccessfn : option P.AffineFnT := P.composeAffineFunction
-                                   (scopStmtAccessFunction ss)
-                                   (scopStmtSchedule ss) in *)
+  Definition evalAccessFunction (se: ScopEnvironment) (viv : P.PointT)
+             (accessfn: P.AffineFnT): option (list Z) := Some [].
     
-    let oaccessfn : option P.AffineFnT := 
-        Some (scopStmtAccessFunction ss) in
-
-    let viv : P.PointT := scopenvVIV se in
-    
-    let oiv : option P.PointT := oaccessfn >>= fun f => P.mapPoint f viv in
-    let oaccessix : option (list Z) :=
-        oiv >>= fun iv => P.evalPoint (scopenvParams se) iv in
-    match (oaccessix, scopStmtType ss)  with
-    | (Some accessix, SSTstore val) => storeArray
-                                         (scopStmtArrayIdent ss)
-                                         accessix
-                                         (val accessix)
-                                         se
-                                         mem
-    | (Some accessix, SSTload) => mem
-    | (None, _) => mem
-    end.
-
-
-  (* 
-    (* Add a new induction varible into the environment, replacing
-the previous value of the induction variable (if it existed ) *)
-    Definition setIndvarInEnv (env: Environment)
-               (indvar: Indvar)
-               (val: Value) : Environment :=
-      let ivToValue : ZMap.t (option Value) := envIndvarToValue env in
-      let newIvToValue := ZMap.set indvar (Some (val%Z)) ivToValue in
-      {|
-        envIndvarToValue := newIvToValue; 
-        envIdentToChunkNum := envIdentToChunkNum env;
-        envLoopDepth := envLoopDepth env
-      |}.
-   *)
-
-  (* 
-    (* If the list of affine expressions are valid: that is, expression at index J only refers to variables in indeces 0 <= i < J,
-then this will return a valid list of bounds. Note that usually,
- domain expressions need to be evaluated this way to find domains.
- However, objects such as general affine expressions should not be
- evaluated this way! *)
-    Fixpoint getMultidimAffineExprExtent
-             (env: Environment)
-             (ivs: list Indvar)
-             (aes: MultidimAffineExpr)
-      :  list (option Value) :=
-      match (ivs, aes) with
-      | (_, []) =>  []
-      | ([], _) => []
-      | (iv::ivs', ae::aes') =>
-        let oval := evalAffineExprFn env ae in
-        match oval with
-        | None => []
-        | Some val =>
-          let env' := setIndvarInEnv env iv val in
-          (Some val)::(getMultidimAffineExprExtent env' ivs' aes')
-        end
-      end.
-   *)
-  
-  
-
-  (** Get the statements whose domain is contained in the current environment **)
-  Definition getActiveScopStmtsInScop (s: Scop)
-             (se: ScopEnvironment): list ScopStmt :=
-    List.filter (isScopStmtActive se) (scopStmts s).
-
-  (** Run a scop for a step with some given environment and memory. **)
-  Definition runScopStepWithEnvAndMem (s: Scop)
-             (se: ScopEnvironment)
-             (mem: Memory) : Memory :=
-    List.fold_left (fun m ss => runScopStmt ss se m)
-                   (getActiveScopStmtsInScop s se) mem.
-
-
 
 
   (* 
@@ -641,115 +560,32 @@ then this will return a valid list of bounds. Note that usually,
    *)
 
   
-  Definition setVIVInScopEnv (vivs: P.PointT)
-             (se: ScopEnvironment):ScopEnvironment :=
-    {|
-      scopenvVIV := vivs;
-      scopenvParams := scopenvParams se;
-      scopenvIdentToChunkNum := scopenvIdentToChunkNum se;
-    |}.
-  
-
-  (* Try to bump up the induction variable values, and give up
-    if it is not possible *)
-  Definition bumpScopenvVIV
-             (scopDomain: P.PolyT)
-             (se: ScopEnvironment)
-    : option ScopEnvironment :=
-    option_map (fun viv' => setVIVInScopEnv viv' se)
-               (P.getNextLexLargerPoint (scopenvParams se)
-                                        (scopDomain)
-                                        (scopenvVIV se)).
-  
-  (** update all the environment induction variables to their next value **)
-  (** This is separate from bumpEnvindvarvalues for conceptual clarity.
-Could be merged later... **)
-  Definition stepScopenv
-             (scopDomain: P.PolyT)
-             (se: ScopEnvironment) : option ScopEnvironment
-    := bumpScopenvVIV scopDomain se.
 
 
-  (* Note that the fuel is OK, we can calculate how much fuel to provide
-based on the domain extent *)
-  Fixpoint runScop_
-           (fuel: nat)
-           (scopDomain: P.PolyT)
-           (se: ScopEnvironment)
-           (mem: Memory)
-           (s: Scop)
-           {struct fuel}: ScopEnvironment * Memory :=
-    let mem' := runScopStepWithEnvAndMem s se mem in
-    let ose' := stepScopenv scopDomain se in
-    match fuel with
-    | O => (se, mem)
-    | S fuel' => 
-      match ose' with
-      | None => (se, mem)
-      | Some se' => runScop_ fuel' scopDomain se' mem' s
-      end
-    end.
-  
+  Definition getMemAccessLoadRelation (ma: MemoryAccess) : P.AffineRelT :=
+    match ma with
+    | MALoad _ accessfn => P.affineFnToAffineRel accessfn
+    | _  =>  P.emptyAffineRel
+    end .
 
-  (* 
-    Definition maxListPointwise (l1 l2: list Value): list Value :=
-      zipWith Z.max l1 l2.
-
-    Check (fold_left).
-    Definition fold_left_1 {X: Type} (f: X -> X -> X) (xs: list X): option X :=
-      match xs with
-      | [] => None
-      | x:: xs => Some (fold_left f xs x)
-      end.
+  Definition getMemAccessStoreRelation (ma: MemoryAccess) : P.AffineRelT :=
+    match ma with
+    | MAStore _ accessfn _ => P.affineFnToAffineRel accessfn
+    | _=>  P.emptyAffineRel
+    end .
+                                        
 
 
-    (* Get the union of the domains of all the individual scops *)
-    Definition getScopDomainExtent (initenv: Environment) (s: Scop):
-      option (list Value) :=
-      let odoms : option (list (list Value)) :=
-          option_traverse (List.map
-                             (fun ss => option_traverse
-                                       ((getMultidimAffineExprExtent
-                                           initenv
-                                           (scopStmtIndvars ss)
-                                           (scopStmtDomain ss)))) (scopStmts s))
-      in match odoms with
-         | None => None
-         | Some doms => fold_left_1 maxListPointwise doms
-         end.
-
-    Definition getNumPointsInExtent (extent: list Value): Value :=
-      fold_left Z.mul extent 1%Z.
-   *)
-
-  Check (List.fold_left).
-  Definition getScopDomain  (s: Scop) : option P.PolyT :=
-    let domains: list (P.PolyT) := List.map scopStmtDomain (scopStmts s) in
-    fold_left (fun op q => op >>= fun p => P.unionPoly p q) domains (Some P.emptyPoly) .
-  
-  
-  Definition runScop (s: Scop)
-             (se: ScopEnvironment)
-             (initmem: Memory): option (ScopEnvironment * Memory) :=
-    getScopDomain s >>=
-                  fun dom => P.getOverapproximationNumPointsInPoly
-                               (scopenvParams se)
-                               dom >>= fun fuel =>
-                                         Some (runScop_ fuel dom se initmem s).
-
-
-  
+  (* TODO: intersect with the domain of the scop statement *)
   Definition getScopStmtLoads (ss: ScopStmt): P.AffineRelT :=
-    match scopStmtType ss with
-    | SSTstore _ => P.emptyAffineRel
-    | SSTload =>  P.affineFnToAffineRel (scopStmtAccessFunction ss)
-    end.
+    List.fold_left P.unionAffineRel
+                   (List.map getMemAccessLoadRelation  (scopStmtMemAccesses ss))
+                   P.emptyAffineRel.
 
   Definition getScopStmtStores (ss: ScopStmt): P.AffineRelT :=
-    match scopStmtType ss with
-    | SSTload => P.emptyAffineRel
-    | SSTstore _ =>  P.affineFnToAffineRel (scopStmtAccessFunction ss)
-    end.
+    List.fold_left P.unionAffineRel
+                   (List.map getMemAccessStoreRelation  (scopStmtMemAccesses ss))
+                   P.emptyAffineRel.
   
   Definition getScopStores(s: Scop): P.AffineRelT :=
     List.fold_left (fun rel ss =>
@@ -790,15 +626,14 @@ based on the domain extent *)
       scheduleRespectsDependence schedule rel.
 
 
+
   Definition applyScheduleToScopStmt
              (schedule: P.AffineFnT)
              (ss: ScopStmt): option ScopStmt :=
     option_map (fun newschedule => {|
-                    scopStmtArrayIdent := scopStmtArrayIdent ss;
                     scopStmtDomain:= scopStmtDomain ss;
                     scopStmtSchedule := newschedule;
-                    scopStmtAccessFunction := scopStmtAccessFunction ss;
-                    scopStmtType := scopStmtType ss
+                    scopStmtMemAccesses := scopStmtMemAccesses ss
                   |}) (P.composeAffineFunction (scopStmtSchedule ss) schedule).
 
   Definition applyScheduleToScop
@@ -831,170 +666,100 @@ based on the domain extent *)
   Hint Resolve applyScheduleToScopStmt_preserves_scop_stmt_domain.
   Hint Rewrite applyScheduleToScopStmt_preserves_scop_stmt_domain.
 
-  Lemma getScopDomain_cons: forall (ss : ScopStmt)
-                                   (sslist: list ScopStmt)
-                                   sindvar,
-      getScopDomain {| scopStmts := ss :: sslist; scopIndvars := sindvar |} =
-      getScopDomain {| scopStmts := sslist; scopIndvars := sindvar; |}.
-  Proof.
-  Abort.
-
-  Lemma applyScheduleToScopStmt_access_fn_eq:
-    forall (ss ss': ScopStmt)
-           (schedule: P.AffineFnT)
-           (MAPPED: applyScheduleToScopStmt schedule ss = Some ss'),
-      scopStmtAccessFunction ss = scopStmtAccessFunction ss'.
-  Proof.
-    intros.
-    unfold applyScheduleToScopStmt in *.
-    destruct (P.composeAffineFunction (scopStmtSchedule ss) schedule);
-      simpl in MAPPED;
-      inversion MAPPED;
-      auto.
-  Qed.
-
-  Hint Resolve applyScheduleToScopStmt_access_fn_eq.
-  Hint Rewrite applyScheduleToScopStmt_access_fn_eq.
-
-  
-  
-  Lemma applyScheduleToScop_scop_domain_eq:
-    forall (scop scop': Scop)
-           (schedule: P.AffineFnT)
-           (MAPPED: applyScheduleToScop schedule scop = Some scop'),
-      getScopDomain scop = getScopDomain scop'.
-  Proof.
-    intros.
-    destruct scop as [ss sindvar].
-    induction ss; simpl in *.
-    - (* base case *)
-      unfold applyScheduleToScop in MAPPED.
-      inversion MAPPED.
-      auto.
-
-    - simpl in MAPPED.
-  Admitted.
-  
-  Hint Resolve applyScheduleToScop_scop_domain_eq.
-  Hint Rewrite applyScheduleToScop_scop_domain_eq.
-
-  
-  Lemma isScopStmtActive_eq: forall (se: ScopEnvironment)
-                                    (ss ss': ScopStmt)
-                                    (schedule: P.AffineFnT)
-                                    (MAPPEDSS: Some ss' =
-                                               applyScheduleToScopStmt schedule ss),
-      isScopStmtActive se ss = isScopStmtActive se ss'.
-  Proof.
-    intros.
-    unfold isScopStmtActive.
-    eauto.
-  Qed.
-  Hint Resolve isScopStmtActive_eq.
-  Hint Rewrite isScopStmtActive_eq.
-  
-  
-  
-  
-  
-  Section SEMANTICS_PRESERVATION_PROOF.
-    (** Preservation properties of applyScheduleToScop **)
-    Variable schedule: P.AffineFnT.
-    Variable scop scop': Scop.
-
-    Variable RESPECTRAW: scheduleRespectsRAW schedule scop.
-    Variable RESPECTWAW: scheduleRespectsWAW schedule scop.
-    Variable MAPPED: applyScheduleToScop schedule scop = Some scop'.
-
+    
+    (* Check if the current value of the induction variables is within
+the scop stmts domain *)
+    Definition isScopStmtActive (viv: P.PointT) (ss: ScopStmt) : bool :=
+      P.isPointInPoly viv (scopStmtDomain ss).
 
     
-    Lemma getActiveScopStmtsInScop_eq:
-      forall (se: ScopEnvironment),
-      exists (ss': list ScopStmt),
-        option_traverse (List.map (applyScheduleToScopStmt schedule)
-                                  (getActiveScopStmtsInScop scop se)) = Some ss' /\
-        getActiveScopStmtsInScop scop' se = ss'.
-    Proof.
-      intros.
-      unfold getActiveScopStmtsInScop.
-    Admitted.
-    
-    
-    Lemma runScopStepWithEnvAndMem_eq:
-      forall (se: ScopEnvironment)
-             (mem: Memory),
-        runScopStepWithEnvAndMem scop se mem = runScopStepWithEnvAndMem
-                                                 scop' se mem.
-    Proof.
-      intros.
-      unfold runScopStepWithEnvAndMem.
-
-      assert (ACTIVE_STMTS_IN_SCOP': exists ss': list ScopStmt,
-                 option_traverse
-                   (List.map (applyScheduleToScopStmt schedule)
-                             (getActiveScopStmtsInScop scop se)) =
-                 Some ss' /\
-                 getActiveScopStmtsInScop scop' se = ss'
-             ).
-      admit.
-
-      destruct ACTIVE_STMTS_IN_SCOP' as [ss' [SS' ACTIVE_IN_SCOP']].
-      rewrite ACTIVE_IN_SCOP'.
-
-      remember (getActiveScopStmtsInScop scop se) as ss eqn:ACTIVE_IN_SCOP.
-
-      (* Induction on the scop statements themseleves *)
-      induction ss.
-
-      - simpl in *. inversion SS'. auto.
-      - 
-    Admitted.
-
-    Hint Resolve runScopStepWithEnvAndMem_eq.
-
-    
-    Theorem runScop_eq:
-      forall (fuel: nat)
-        (se: ScopEnvironment)
-        (initmem: Memory)
-        (scopdom: P.PolyT)
-        (SCOPDOMAIN: Some scopdom = getScopDomain scop'),
-        runScop_ fuel scopdom se initmem scop =
-        runScop_ fuel scopdom se initmem scop'.
-    Proof.
-      intros fuel.
-      induction fuel; intros; auto.
-      - simpl.
-        destruct (stepScopenv scopdom se) eqn:SCOPENV'; auto.
-        rewrite runScopStepWithEnvAndMem_eq.
-        apply IHfuel; auto.
-    Qed.
-
-    Hint Resolve runScop_eq.
-
-
-    (* Main theorem: Applying a valid schedule on a scop preserves
-    the semantics of the scop *)
-    Theorem applying_valid_schedule_preserves_semantics:
-      forall (se: ScopEnvironment)
-        (initmem: Memory),
-        runScop scop se initmem = runScop scop' se initmem.
-    Proof.
-      intros.
-      unfold runScop.
+  Definition runMemoryAccess (se: ScopEnvironment)
+             (viv: P.PointT)
+             (memacc: MemoryAccess)
+             (mem: Memory): option Memory :=
+    match memacc with
+    | MAStore name accessfn valfn  =>
       
-      erewrite applyScheduleToScop_scop_domain_eq; eauto.
-      destruct (getScopDomain scop') eqn:SCOPDOMAIN;  auto.
-      rename p into scopdom.
-      simpl.
+      option_map (fun accessix => storeArray name
+                                   accessix
+                                   (valfn accessix)
+                                   se
+                                   mem)
+                 (evalAccessFunction se viv accessfn)
+    | MALoad  _ _=> None
+    end.
+                 
+  
+  (** TODO: make loads an actual statement in the PolyIR language **)
+  Definition evalScopStmt (ss: ScopStmt)
+             (viv: P.PointT)
+             (se: ScopEnvironment)
+             (initmem: Memory) : option Memory :=
 
-      destruct (P.getOverapproximationNumPointsInPoly (scopenvParams se) scopdom)
-               eqn:FUEL; auto.
-      rename n into fuel.
-      simpl; auto.
-    Qed.
+    option_traverse_fold_left initmem
+                              (fun mem memacc => runMemoryAccess se viv memacc mem)
+                              (scopStmtMemAccesses ss).
+  
+  
 
-  End SEMANTICS_PRESERVATION_PROOF.
+  (** Get the statements whose domain is contained in the current environment **)
+  Definition getActiveScopStmtsInScop
+             (s: Scop)
+             (viv: P.PointT)
+             : list ScopStmt :=
+    List.filter (isScopStmtActive viv) (scopStmts s).
+
+      
+
+
+  Definition evalPointInScop (s: Scop)
+             (se: ScopEnvironment)
+             (viv: P.PointT)
+             (initmem: Memory): option Memory :=
+    option_traverse_fold_left
+      initmem (fun m ss => evalScopStmt ss viv se m)
+      (getActiveScopStmtsInScop s viv) .
+    
+    
+  Fixpoint evalPointsInScopFromVIV
+           (scop: Scop)
+           (scopDomain: P.PolyT)
+           (params: P.ParamsT)
+           (se: ScopEnvironment)
+           (viv: P.PointT)
+           (mem: Memory)
+           (fuel: nat): option Memory :=
+    match fuel with
+    | O => None
+    | S fuel' =>
+      evalPointInScop scop se  viv mem >>=
+                      (fun mem' => match P.getNextLexPoint params scopDomain viv with
+                                | None => Some mem'
+                                | Some viv' =>evalPointsInScopFromVIV scop
+                                                                     scopDomain
+                                                                     params
+                                                                     se
+                                                                     viv'
+                                                                     mem'
+                                                                     fuel'
+                                end)
+    end.
+
+  Definition getScopDomain (scop: Scop): P.PolyT. Admitted.
+  Definition getScopFuel (scop: Scop): nat. Admitted.
+  
+  Definition evalScop (scop: Scop)
+             (se: ScopEnvironment)
+             (params: P.ParamsT)
+             (mem: Memory) : option Memory := evalPointsInScopFromVIV
+                           scop
+                           (getScopDomain scop)
+                           params
+                           se
+                           (P.getLexminPoint params (getScopDomain scop))
+                           mem
+                           (getScopFuel scop).
+  
 
   
 End SCOP.
